code/experimental/P256/Hacl.Impl.P256.fsti
@@ -141,6 +141,13 @@ val norm: p: point -> resultPoint: point -> tempBuffer: lbuffer uint64 (size 88)
    )   
   )
 
+
+val isPointAtInfinityPrivate: p: point -> Stack uint64
+  (requires fun h -> live h p)
+  (ensures fun h0 r h1 -> modifies0 h0 h1) 
+
+
+
 inline_for_extraction noextract
 val scalarMultiplication: #buf_type: buftype->  p: point -> result: point -> 
   scalar: lbuffer_t buf_type uint8 (size 32) -> 
@@ -179,7 +186,6 @@ val secretToPublic: result: point -> scalar: lbuffer uint8 (size 32) ->
   )  
 
 
-
 val isPointAtInfinity: p: point -> Stack bool
   (requires fun h -> live h p)
   (ensures fun h0 r h1 -> modifies0 h0 h1 /\ 
@@ -206,7 +212,7 @@ val isPointOnCurve: p: point -> Stack bool
       let y = gsub p (size 4) (size 4) in 
       let x_ = as_nat h0 x in  if r = false then (as_nat h0 y) * (as_nat h0 y) % prime <>  (x_ * x_ * x_ - 3 * x_ - 41058363725152142129326129780047268409114441015993725554835256314039467401291) % prime
        else
-       (as_nat h0 y) * (as_nat h0 y) % prime == (x_ * x_ * x_ - 3 * x_ - 41058363725152142129326129780047268409114441015993725554835256314039467401291) % prime) /\
+       (as_nat h0 y) * (as_nat h0 y) % prime == (x_ * x_ * x_ - 3 * x_ + 41058363725152142129326129780047268409114441015993725554835256314039467401291) % prime) /\
   r == isPointOnCurve (
   as_nat h1 (gsub p (size 0) (size 4)), as_nat h1 (gsub p (size 4) (size 4)), as_nat h1 (gsub p (size 8) (size 4))
   ) 
